src/tls/Mem.fst
@@ -17,6 +17,7 @@ module HH = FStar.HyperHeap // avoid if we can
 module HS = FStar.HyperStack
 //module ST = FStar.HyperStack.ST
 
+let disjoint = HH.disjoint 
 
 //type fresh_subregion r0 r h0 h1 = ST.stronger_fresh_region r h0 h1 /\ ST.extends r r0
 
@@ -48,21 +49,94 @@ type fresh_subregion child parent h0 h1 =
 type subrgn parent = r:rgn{HH.parent r = parent}
 
 /// Global top-level region for TLS ideal state.
-/// (why do we need a subregion for tables?)
 ///
+/// Top-level disjointness is awkward; we could instead maintain a
+/// private mutable set of regions known to be pairwise-distinct.
+/// 
 let tls_region: tls_rgn = new_colored_region HH.root tls_color
 
-private let p : r:subrgn tls_region{is_tls_rgn r}
-              & r':subrgn tls_region{is_tls_rgn r' /\ r' `HH.disjoint` r}
-             & r'':subrgn tls_region{is_tls_rgn r'' /\ r'' `HH.disjoint` r' /\ r'' `HH.disjoint` r} =
-  let r = new_colored_region tls_region tls_color in
-  let r' = new_colored_region tls_region tls_color in
-  let r'' = new_colored_region tls_region tls_color in
-  (| r, r', r'' |)
+type subtls = r: subrgn tls_region {is_tls_rgn r}
 
+private let p : r0: subtls & r1: subtls & r2: subtls 
+  {r1 `disjoint` r0 /\ r2 `disjoint` r0 /\ r2 `disjoint` r1} =
+  let r0 = new_colored_region tls_region tls_color in
+  let r1 = new_colored_region tls_region tls_color in
+  let r2 = new_colored_region tls_region tls_color in
+  (| r0, r1, r2 |)
+
+// consider dropping the tls_ prefix
 let tls_tables_region: r:tls_rgn =
   match p with | (| r, _, _ |) -> r
-let tls_define_region: r:tls_rgn{r `HH.disjoint` tls_tables_region} =
+let tls_define_region: r:tls_rgn{r `disjoint` tls_tables_region} =
   match p with | (| _, r, _ |) -> r
-let tls_honest_region: r:tls_rgn{r `HH.disjoint` tls_tables_region /\ r `HH.disjoint` tls_define_region} =
+let tls_honest_region: r:tls_rgn{r `disjoint` tls_tables_region /\ r `disjoint` tls_define_region} =
   match p with | (| _, _, r |) -> r
+
+
+// FIXME(adl) can't write Set.set rgn because unification fails in pkg!!
+// FIXME(adl) overcomplicated type because of transitive modifications.
+// An rset can be thought of as a set of disjoint subtrees in the region tree
+// the second line embeds the definition of rgn because of the unification bug
+type rset = s:Set.set HH.rid{
+  (forall (r1:rgn) (r2:rgn).{:pattern (Set.mem r1 s /\ Set.mem r2 s)} (Set.mem r1 s /\ Set.mem r2 s) ==> (r1 == r2 \/ HH.disjoint r1 r2)) /\
+  (forall (r1:rgn). (Set.mem r1 s ==>
+     r1<>HH.root /\
+     (is_tls_rgn r1 ==> r1 `HH.extends` tls_tables_region) /\
+     (forall (s:HH.rid).{:pattern is_eternal_region s} s `is_above` r1 ==> is_eternal_region s)))}
+
+// We get from the definition of rset that define_region and tls_honest_region are disjoint
+let lemma_define_tls_honest_regions (s:rset)
+  : Lemma (~(Set.mem tls_define_region s) /\ ~(Set.mem tls_honest_region s))
+  = ()
+
+//  if Set.mem tls_define_region s then
+//    assert(tls_define_region `HH.extends` tls_)
+
+type disjoint_rset (s1:rset) (s2:rset) =
+  Set.disjoint s1 s2 /\
+  (forall (r1:rgn) (r2:rgn).{:pattern (Set.mem r1 s1 /\ Set.mem r2 s2)}
+   (Set.mem r1 s1 /\ Set.mem r2 s2) ==> HH.disjoint r1 r2)
+
+assume val lemma_disjoint_ancestors:
+  r1:rgn -> r2:rgn -> p1:rgn{r1 `is_below` p1} -> p2:rgn{r2 `is_below` p2}
+  -> Lemma (requires p1 <> p2) (ensures HH.disjoint r1 r2 /\ r1 <> r2)
+
+
+(* Definedness *)
+
+module MM = FStar.Monotonic.Map
+module MR = FStar.Monotonic.RRef
+
+let model = Flags.model
+
+
+// FIXME(adl) extend MonotoneMap
+let mm_fold 
+  (#r:MR.rid) (#a:Type) (#b:a -> Type) (#inv:MM.map' a b -> Type0) (t:MM.t r a b inv)
+  (#rt:Type) (init:rt) (folder: rt -> i:a -> b i -> GTot rt) (h:mem): GTot rt
+ = admit()
+
+type mm_forall 
+  (#r:MR.rid) (#a:Type) (#b:a -> Type) (#inv:MM.map' a b -> Type0) (t:MM.t r a b inv) 
+  (phi: #i:a -> b i -> mem -> GTot Type0) (h:mem) =
+   forall (i:a).{:pattern (MM.defined t i h)}
+     MM.defined t i h ==>
+       (let k = Some?.v (MM.sel (MR.m_sel h t) i) in phi k h)
+
+let lemma_forall_frame 
+  (#r:MR.rid) (#a:Type) (#b:a -> Type) (#inv:MM.map' a b -> Type0) (t:MM.t r a b inv) 
+  (phi: #i:a -> b i -> mem -> GTot Type0)
+  (footprint: #i:a -> v:b i -> GTot rset)
+  (phi_frame: r:HH.rid -> i:a -> h0:mem -> v:b i -> h1:mem ->
+    Lemma (requires phi v h0 /\ modifies_one r h0 h1 /\ ~(Set.mem r (footprint v)))
+          (ensures phi v h1))
+  (r:HH.rid) 
+  (h0:mem) 
+  (h1:mem): Lemma 
+  (requires 
+    mm_forall t phi h0 /\ 
+    (modifies_one r h0 h1 \/ modifies_none h0 h1) /\
+    (forall (i:a) (v:b i). ~(r `Set.mem` footprint v)))
+  (ensures mm_forall t phi h1)
+= 
+  admit()
